Optimizations/DSL/ConditionDSL.thy
@@ -1,0 +1,419 @@
+theory ConditionDSL
+  imports CodeGenAlt JavaAST
+  keywords
+    "register_method" :: thy_decl and
+    "define_semantics" :: thy_decl
+begin
+
+type_synonym ClassName = String.literal
+
+fun unary_op_class :: "IRUnaryOp \<Rightarrow> ClassName" where
+  "unary_op_class UnaryAbs = STR ''AbsNode''" |
+  "unary_op_class UnaryNeg = STR ''NegateNode''" |
+  "unary_op_class UnaryNot = STR ''NotNode''" |
+  "unary_op_class UnaryLogicNegation = STR ''LogicNegationNode''" |
+  "unary_op_class (UnaryNarrow _ _) = STR ''NarrowNode''" |
+  "unary_op_class (UnarySignExtend _ _) = STR ''SignExtendNode''" |
+  "unary_op_class (UnaryZeroExtend _ _) = STR ''ZeroExtendNode''" |
+  "unary_op_class UnaryIsNull = STR ''IsNullNode''" |
+  "unary_op_class UnaryReverseBytes = STR ''ReverseBytesNode''" |
+  "unary_op_class UnaryBitCount = STR ''BitCountNode''"
+
+fun binary_op_class :: "IRBinaryOp \<Rightarrow> ClassName" where
+  "binary_op_class BinAdd = STR ''AddNode''" |
+  "binary_op_class BinMul = STR ''MulNode''" |
+  "binary_op_class BinSub = STR ''SubNode''" |
+  "binary_op_class BinAnd = STR ''AndNode''" |
+  "binary_op_class BinOr = STR ''OrNode''" |
+  "binary_op_class BinXor = STR ''XorNode''" |
+  "binary_op_class BinShortCircuitOr = STR ''ShortCircuitOrNode''" |
+  "binary_op_class BinLeftShift = STR ''LeftShiftNode''" |
+  "binary_op_class BinRightShift = STR ''RightShiftNode''" |
+  "binary_op_class BinURightShift = STR ''UnaryRightShiftNode''" |
+  "binary_op_class BinIntegerEquals = STR ''IntegerEqualsNode''" |
+  "binary_op_class BinIntegerLessThan = STR ''IntegerLessThanNode''" |
+  "binary_op_class BinIntegerBelow = STR ''IntegerBelowNode''" |
+  "binary_op_class BinIntegerTest = STR ''IntegerTestNode''" |
+  "binary_op_class BinIntegerNormalizeCompare = STR ''IntegerNormalizeCompareNode''" |
+  "binary_op_class BinIntegerMulHigh = STR ''IntegerMulHighNode''"
+
+fun class_name :: "IRExpr \<Rightarrow> ClassName option" where
+  "class_name (UnaryExpr op v) = Some (unary_op_class op)" |
+  "class_name (BinaryExpr op v1 v2) = Some (binary_op_class op)" |
+  "class_name (ConditionalExpr v1 v2 v3) = Some (STR ''ConditionalNode'')" |
+  "class_name (ConstantExpr _) = Some (STR ''ConstantNode'')" |
+  "class_name _ = None"
+
+fun stamp_class_name :: "Stamp \<Rightarrow> ClassName" where
+  "stamp_class_name (IntegerStamp b l h) = STR ''IntegerStamp''" |
+  "stamp_class_name (VoidStamp) = STR ''VoidStamp''" |
+  "stamp_class_name (KlassPointerStamp x y) = STR ''KlassPointerStamp''" |
+  "stamp_class_name (MethodCountersPointerStamp x y) = STR ''MethodCountersPointerStamp''" |
+  "stamp_class_name (MethodPointersStamp x y) = STR ''MethodPointersStamp''" |
+  "stamp_class_name (ObjectStamp _ _ _ _) = STR ''ObjectStamp''" |
+  "stamp_class_name (RawPointerStamp _ _) = STR ''RawPointerStamp''" |
+  "stamp_class_name (IllegalStamp) = STR ''IllegalStamp''"
+
+datatype Condition =
+  Unary IRUnaryOp Condition |
+  Binary IRBinaryOp Condition Condition |
+  Conditional Condition Condition Condition |
+  Constant int |
+  Value Value |
+  Variable String.literal |
+  Expr IRExpr |
+  Stamp Stamp |
+
+  Combine Condition Condition ("_; _") |
+
+  InstanceOf Condition String.literal |
+  Method Condition String.literal "Condition list"
+
+inductive coerce_to_bool :: "Condition \<Rightarrow> bool \<Rightarrow> bool" where
+  "coerce_to_bool (Constant num) (num > 0)" |
+  "coerce_to_bool (Value val) (val_to_bool val)" |
+  "coerce_to_bool lhs lhs' \<and> coerce_to_bool rhs rhs' \<Longrightarrow> coerce_to_bool (Combine lhs rhs) (lhs' \<and> rhs')"
+
+inductive base_semantics :: "Condition \<Rightarrow> Condition \<Rightarrow> bool" where
+  "base_semantics e (Value v) \<and> res = (unary_eval op v) \<Longrightarrow> base_semantics (Unary op e) (Value res)" |
+  "base_semantics x (Value xv) \<and> base_semantics y (Value yv) \<and> res = (bin_eval op xv yv) 
+    \<Longrightarrow> base_semantics (Binary op x y) (Value res)" |
+  "base_semantics c c' \<and> base_semantics t t' \<and> base_semantics f f' \<and> coerce_to_bool c con
+    \<Longrightarrow> base_semantics (Conditional c t f) (if con then t' else f')" |
+  "base_semantics (Constant v') (Value (IntVal 32 (word_of_int v')))" |
+  "base_semantics (Value v) (Value v)" |
+  "base_semantics (Expr e) (Expr e)" |
+  "base_semantics (Stamp s) (Stamp s)" |
+  "base_semantics lhs lhs' \<and> base_semantics rhs rhs' \<Longrightarrow> base_semantics (Combine lhs rhs) (Combine lhs' rhs')" |
+  "base_semantics e (Expr e') \<and> class_name e' = Some class \<Longrightarrow> base_semantics (InstanceOf e class) (Value (IntVal 32 1))" |
+  "base_semantics e (Expr e') \<and> class_name e' \<noteq> Some class \<Longrightarrow> base_semantics (InstanceOf e class) (Value (IntVal 32 0))" |
+  "base_semantics e (Stamp s) \<and> stamp_class_name s = class \<Longrightarrow> base_semantics (InstanceOf e class) (Value (IntVal 32 1))" |
+  "base_semantics e (Stamp s) \<and> stamp_class_name s \<noteq> class \<Longrightarrow> base_semantics (InstanceOf e class) (Value (IntVal 32 0))"
+
+syntax
+  "_method" :: "Condition \<Rightarrow> any \<Rightarrow> args => Condition" ("_.._'(_')" 45)
+  "_method_empty" :: "Condition \<Rightarrow> any => Condition" ("_.._'(')" 45)
+  "_method_syntax" :: "Condition \<Rightarrow> any \<Rightarrow> args => Condition"
+
+translations
+  "i..m(x, xs)" \<rightharpoonup> "_method_syntax i m (x#[xs])"
+  "i..m(x)" \<rightharpoonup> "_method_syntax i m (x#[])"
+  "i..m()" \<rightharpoonup> "_method_syntax i m ([])"
+
+ML \<open>
+fun first_free trm =
+  (case trm of
+    (x $ y) => (case (first_free x) of NONE => first_free y | SOME n => SOME n)
+    | Free (str, _) => SOME str
+    | _ => NONE);
+
+fun isabelle_string ctxt str = Syntax.read_term ctxt ("STR ''" ^  str ^ "''")
+
+fun parse_method ctxt [obj, method, args] =
+  let
+    val method_name = (case (first_free method) of 
+      NONE => raise TERM ("cannot parse method name", [method]) | 
+      SOME name => name);
+    
+    val method_string = (isabelle_string ctxt method_name);
+  in
+    @{term "Method"} $ obj $ method_string $ args
+  end
+  | parse_method _ ts = raise TERM ("markup_expr", ts)
+\<close>
+
+parse_translation \<open> [( @{syntax_const "_method_syntax"} , parse_method)] \<close>
+
+ML_val \<open>@{term "x..stamp(a, b, c, d)"}\<close>
+value "x..stamp(a, b, c)"
+
+syntax
+  "_instanceof" :: "Condition \<Rightarrow> id_position => Condition" ("_ instanceof _")
+
+ML \<open>
+fun parse_instanceof ctxt [obj, class] =
+  let
+    val class_name = (case (first_free class) of 
+      NONE => raise TERM ("cannot parse class name", [class]) | 
+      SOME name => name);
+    
+    val class_string = (isabelle_string ctxt class_name);
+  in
+    @{term "InstanceOf"} $ obj $ class_string
+  end
+  | parse_instanceof _ ts = raise TERM ("markup_expr", ts)
+\<close>
+
+parse_translation \<open> [( @{syntax_const "_instanceof"} , parse_instanceof)] \<close>
+
+(*
+bundle condition_syntax
+begin
+
+notation
+  not  (\<open>NOT\<close>)
+    and "and"  (infixr \<open>AND\<close> 64)
+    and or  (infixr \<open>OR\<close>  59)
+    and xor  (infixr \<open>XOR\<close> 59)
+
+end
+*)
+
+ML \<open>
+fun semantics_code _ name rule =
+  @{const Trueprop} 
+  $ ((Const ("HOL.eq", @{typ "(Condition \<Rightarrow> Condition list \<Rightarrow> Condition) \<Rightarrow> (Condition \<Rightarrow> Condition list \<Rightarrow> Condition) \<Rightarrow> bool"})
+  $ (Free ((Binding.name_of (name)) ^ "_semantics", @{typ "(Condition \<Rightarrow> Condition list \<Rightarrow> Condition)"}))
+  $ rule))
+
+fun translation_code _ name rule =
+  @{const Trueprop} 
+  $ ((Const ("HOL.eq", @{typ "(string \<Rightarrow> string list \<Rightarrow> string) \<Rightarrow> (string \<Rightarrow> string list \<Rightarrow> string) \<Rightarrow> bool"})
+  $ (Free ((Binding.name_of (name)) ^ "_translation", @{typ "(string \<Rightarrow> string list \<Rightarrow> string)"}))
+  $ rule))
+
+structure MethodData = Theory_Data
+(
+  type T = string list;
+  val empty = [];
+  fun merge (lhs, rhs) = lhs @ rhs
+);
+
+val state = MethodData.get;
+
+fun register_method_cmd name semantics translation thy =
+  let
+    val semantics_term = (Syntax.parse_term thy semantics);
+    val (_, thy') = Specification.definition
+      NONE [] []
+      ((Binding.suffix_name "_semantics" (fst name), []), (semantics_code thy (fst name) semantics_term))
+      thy
+
+    val translation_term = (Syntax.parse_term thy translation);
+    val (_, thy'') = Specification.definition
+      NONE [] []
+      ((Binding.suffix_name "_translation" (fst name), []), (translation_code thy (fst name) translation_term))
+      thy'
+
+    val register = (fn state => MethodData.put ((MethodData.get state) @ [Binding.name_of (fst name)]) state);
+    val thy''' = Local_Theory.background_theory register thy'';
+  in
+    thy'''
+  end
+
+val _ =
+  Outer_Syntax.local_theory \<^command_keyword>\<open>register_method\<close>
+    "support a new built-in Java/GraalVM method"
+    (Parse_Spec.thm_name ":" -- Parse.term -- Parse.term
+      >> (fn ((name, semantics), translation) => (register_method_cmd name semantics translation)));
+      (*(fn name => Toplevel.theory (fn state => export_phases state name)))*)
+
+fun rename_const n v (Const (x, T)) =
+        (if x = n then Free (v, T) else Const (x, T))
+    | rename_const n v (Abs (x, T, t)) = (Abs (x, T, rename_const n v t))
+    | rename_const n v (t $ u) = (rename_const n v t $ rename_const n v u)
+    | rename_const _ _ e = e;
+
+fun define_method_call name ctxt method =
+   Const ("Pure.imp", @{typ "prop \<Rightarrow> prop \<Rightarrow> prop"}) $ 
+    (Const ("HOL.Trueprop", @{typ "bool \<Rightarrow> prop"}) $ 
+      (Const ("HOL.conj", @{typ "bool \<Rightarrow> bool \<Rightarrow> bool"}) $
+        (Const ("HOL.conj", @{typ "bool \<Rightarrow> bool \<Rightarrow> bool"}) $
+          (Const ("HOL.eq", @{typ "String.literal \<Rightarrow> String.literal \<Rightarrow> bool"}) $ Free ("name", @{typ "String.literal"}) $ isabelle_string ctxt method) $
+            (Const ("HOL.conj", @{typ "bool \<Rightarrow> bool \<Rightarrow> bool"}) $
+              (Free (name, @{typ "Condition => Condition => bool"}) $ Free ("c", @{typ "Condition"}) $ (Free ("obj", @{typ "Condition"}))) $
+              (Const ("HOL.eq", @{typ "Condition \<Rightarrow> Condition \<Rightarrow> bool"}) $ 
+                Free ("c'", @{typ "Condition"}) $
+                (Const ("ConditionDSL." ^ method ^ "_semantics", @{typ "Condition \<Rightarrow> Condition list \<Rightarrow> Condition"}) 
+                $ Free ("obj", @{typ "Condition"}) $ Free ("params", @{typ "Condition list"})))
+            )
+        ) $
+        (Free (name, @{typ "Condition => Condition => bool"}) $ Free ("c'", @{typ "Condition"}) $ (Free ("c''", @{typ "Condition"})))
+      )) $
+      
+    (Const ("HOL.Trueprop", @{typ "bool \<Rightarrow> prop"}) $
+      (Free (name, @{typ "Condition => Condition => bool"}) 
+        $ (@{term "Method"} $ Free ("c", @{typ "Condition"}) $ Free ("name", @{typ "String.literal"}) $ Free ("params", @{typ "Condition list"}))
+         $ (Free ("c''", @{typ "Condition"}))))
+
+fun define_method_calls name ctxt = map (define_method_call name ctxt)
+
+fun define_semantics_cmd name thy =
+  let
+    val methods = MethodData.get (Proof_Context.theory_of thy);
+    val method_calls = (define_method_calls name thy methods);
+
+    val intrs = map Thm.full_prop_of (#intrs (snd (Inductive.the_inductive thy @{term base_semantics})));
+    val intrs' = map Term.close_schematic_term intrs;
+    val intrs'' = map (rename_const "ConditionDSL.base_semantics" name) intrs';
+    val intrs''' = (map (snd o Term.strip_abs_eta 10) intrs'');
+    val rules = intrs''' @ method_calls;
+    (*val _ = @{print} (Syntax.unparse_term thy intrs''');*)
+    val (res, thy') = (Inductive.add_inductive {quiet_mode = true, verbose = false, alt_name = Binding.name name,
+           coind = false, no_elim = false, no_ind = false, skip_mono = false}
+          (map (fn (s, T) => ((Binding.name s, T), NoSyn)) [(name, @{typ "Condition \<Rightarrow> Condition \<Rightarrow> bool"})])
+          (*([] @ vars)[("c", @{typ Condition}), ("v", @{typ Value})]*) []
+          (*(map dest_Free [@{term \<open>x y\<close>}])*)
+          (map (fn x => (Binding.empty_atts, x)) (rules (*@ [@{term \<open>hello c v \<Longrightarrow> hello (c::Condition) (v::Value)\<close>}]*))) []) thy;
+    val pretty = Pretty.big_list name (map (Syntax.pretty_term thy' o Thm.full_prop_of) (#intrs res));
+    val _ = (fn _ =>
+      Print_Mode.with_modes [] (fn () => writeln (Pretty.string_of pretty)) ()) thy';
+    (*val thy'' = Predicate_Compile.preprocess Predicate_Compile_Aux.default_options (Thm.full_prop_of (#induct res)) thy';*)
+    
+  in
+    thy'
+  end
+
+val _ =
+  Outer_Syntax.local_theory \<^command_keyword>\<open>define_semantics\<close>
+    "construct a new inductive definition of condition semantics"
+    (Parse.name 
+      >> (fn (name) => (define_semantics_cmd name)));
+\<close>
+
+define_semantics myCoolSemantics
+
+thm myCoolSemantics.intros
+
+print_inductives
+
+fun stamp_of :: "Condition \<Rightarrow> Condition list \<Rightarrow> Condition" where
+  "stamp_of (Expr e) _ = Stamp (stamp_expr e)"
+
+fun generate_stamp :: "string \<Rightarrow> string list \<Rightarrow> string" where
+  "generate_stamp e _ = e @ ''.stamp(view)''"
+
+register_method stamp: stamp_of generate_stamp
+
+fun upMask_of :: "Condition \<Rightarrow> Condition list \<Rightarrow> Condition" where
+  "upMask_of (Stamp s) _ = (Constant 0)"
+
+fun generate_upMask :: "string \<Rightarrow> string list \<Rightarrow> string" where
+  "generate_upMask e _ = e @ ''.mayBeSet()''"
+
+register_method upMask: upMask_of generate_upMask
+register_method mayBeSet: upMask_of generate_upMask
+
+fun downMask_of :: "Condition \<Rightarrow> Condition list \<Rightarrow> Condition" where
+  "downMask_of (Stamp s) _ = (Constant 0)"
+
+fun generate_downMask :: "string \<Rightarrow> string list \<Rightarrow> string" where
+  "generate_downMask e _ = e @ ''.mustBeSet()''"
+
+register_method downMask: downMask_of generate_downMask
+register_method mustBeSet: downMask_of generate_downMask
+
+fun lowerBound_of :: "Condition \<Rightarrow> Condition list \<Rightarrow> Condition" where
+  "lowerBound_of (Stamp s) _ = Constant (stpi_lower s)"
+
+fun generate_lowerBound :: "string \<Rightarrow> string list \<Rightarrow> string" where
+  "generate_lowerBound e _ = e @ ''.lowerBound()''"
+
+register_method lowerBound: lowerBound_of generate_lowerBound
+
+fun upperBound_of :: "Condition \<Rightarrow> Condition list \<Rightarrow> Condition" where
+  "upperBound_of (Stamp s) _ = Constant (stpi_upper s)"
+
+fun generate_upperBound :: "string \<Rightarrow> string list \<Rightarrow> string" where
+  "generate_upperBound e _ = e @ ''.upperBound()''"
+
+register_method upperBound: upperBound_of generate_upperBound
+
+define_semantics stampConditions
+
+inductive_cases UnaryCool: "stampConditions (Unary op e) c'"
+inductive_cases BinaryCool: "stampConditions (Binary op x y) c'"
+inductive_cases ConditionalCool: "stampConditions (Conditional c t f) c'"
+
+code_pred (modes: i \<Rightarrow> o \<Rightarrow> bool as execCond) stampConditions .
+
+(*
+lemma semdet:
+  assumes "myCoolSemantics2 c c'"
+  assumes "myCoolSemantics2 c c''"
+  shows "c' = c''"
+  using assms apply (induction c arbitrary: c' c'')
+            apply (metis Condition.inject(5) UnaryCool) 
+  apply (metis BinaryCool Condition.inject(5))
+          apply (smt (verit, best) Condition.distinct(55) Condition.inject(4) Condition.inject(5) ConditionalCool coerce_to_bool.simps)
+  apply (smt (z3) Condition.distinct(59) Condition.distinct(61) Condition.distinct(65) Condition.simps(17) Condition.simps(35) Condition.simps(4) Condition.simps(51) Condition.simps(66) Condition.simps(75) Condition.simps(79) myCoolSemantics2.cases)
+  sorry
+
+experiment begin
+definition e where "e = (Expr (ConstantExpr (IntVal 32 400)))"
+
+value "stamp_semantics e []"
+value "stamp_translation ''e'' []"
+
+values "{c'. myCoolSemantics2 (cond[e..stamp()..upMask()]) c'}"
+values "{c'. myCoolSemantics2 (cond[((e..stamp()..upMask()) & (e..stamp()..upMask()))]) c'}"
+values "{c'. myCoolSemantics2 (cond[((e..stamp()..upMask()) & (e..stamp()..upMask())) eq (const 0)]) c'}"
+value "Predicate.the (execCond (cond[((e..stamp()..upMask()) & (e..stamp()..upMask())) eq (const 0)]))"
+
+values "{c'. myCoolSemantics2 (cond[e..stamp() instanceof IntegerStamp]) c'}"
+value "Predicate.the (execCond (cond[e..stamp() instanceof IntegerStamp]))"
+
+definition x where "x = (Expr (LeafExpr 10 default_stamp))"
+
+values "{c'. myCoolSemantics2 (cond[x instanceof ConstantNode; !(e instanceof ConstantNode)]) c'}"
+value "Predicate.the (execCond (cond[x instanceof ConstantNode; !(e instanceof ConstantNode)]))"
+value "Predicate.the (execCond (cond[e instanceof ConstantNode; !(x instanceof ConstantNode)]))"
+value "Predicate.the (execCond (cond[e instanceof ConstantNode]))"
+
+
+lemma
+  (*assumes "s = Stamp (IntegerStamp 32 400 400)"*)
+  assumes "e = (Expr (ConstantExpr (IntVal 32 400)))"
+  assumes "s = expr_of e []"
+  shows "myCoolSemantics2 (e..stamp()) v = myCoolSemantics2 s v"
+  using assms using myCoolSemantics2.intros(13) unfolding stamp_semantics sorry
+
+register_method stamp2: stamp_of "\<lambda>e _. e @ ''.stamp(view)''"
+
+value "stamp2_translation ''e'' []"
+
+abbreviation "stampe \<equiv> stamp_translation"
+
+inductive hello where "hello x"
+
+print_commands
+end
+*)
+
+context includes java_ast_syntax begin
+(*
+  Unary IRUnaryOp Condition |
+  Binary IRBinaryOp Condition Condition |
+  Conditional Condition Condition Condition |
+  Constant int |
+  Value Value |
+  Variable String.literal |
+  Expr IRExpr |
+  Stamp Stamp |
+
+  Combine Condition Condition ("_; _") |
+
+  InstanceOf Condition String.literal |
+  Method Condition String.literal "Condition list"*)
+
+fun export :: "Condition \<Rightarrow> Expression" where
+  "export (Unary op e) = (JavaUnary op (export e))" |
+  "export (Binary op x y) = (JavaBinary op (export x) (export y))" |
+  (* Conditional - needed? *)
+  "export (Constant v) = (JavaConstant v)" |
+  "export (Value (IntVal _ v)) = (JavaConstant (Word.the_int v))" |
+  "export (Variable v) = (JavaVariable v)" |
+  "export (InstanceOf c cn) = (JavaInstanceOf (export c) cn STR ''_'')" |
+  "export (Method obj mn ps) = (JavaMethodCall (export obj) mn (map export ps))" |
+  "export (Combine lhs rhs) = (JavaBinary BinAnd (export lhs) (export rhs))"
+
+(*
+value "generate_expression (export cond[(Variable STR ''x'') instanceof ConstantNode; !(Variable STR ''y'' instanceof ConstantNode)])"
+value "export cond[x..stamp() instanceof IntegerStamp]"
+value "export cond[((z..stamp()..upMask()) & (y..stamp()..upMask())) eq (const 0)]"
+value "export cond[y..isPowerOf2()]"
+*)
+
+end
+
+end
